More improvement in logic abstraction. Now, precise and mapsto are added into logic level.

msl_ext/seplog.v
@@ -3,6 +3,39 @@ Require Import VST.msl.seplog.
 
 Local Open Scope logic.
 
+Class HONatDed (A: Type) {ND: NatDed A} := mkHONatDed {
+  allp_uncurry: forall (S T: Type) (P: S -> T -> A),
+    allp (fun s => allp (P s)) = allp (fun st => P (fst st) (snd st));
+  allp_curry: forall (S T: Type) (P: S * T -> A),
+    allp P = allp (fun s => allp (fun t => P (s, t)));
+  exp_uncurry: forall (S T: Type) (P: S -> T -> A),
+    exp (fun s => exp (P s)) = exp (fun st => P (fst st) (snd st));
+  exp_curry: forall (S T: Type) (P: S * T -> A),
+    exp P = exp (fun s => exp (fun t => P (s, t)));
+  allp_exp: forall (S T: Type) (P: S -> T -> A),
+    allp (fun s => exp (P s)) = exp (fun t: S -> T => allp (fun s => P s (t s)));
+  exp_allp: forall (S T: Type) (P: S -> T -> A),
+    exp (fun s => allp (P s)) |-- allp (fun t => exp (fun s => P s t))
+}.
+
+Class PreciseSepLog (A: Type) {ND: NatDed A} {SL: SepLog A} := mkPreciseSepLog {
+  precise: A -> Prop;
+  precise_sepcon_andp_sepcon: forall P Q R, precise P -> (P * Q) && (P * R) |-- P * (Q && R);
+  precise_sepcon_cancel: forall P Q R, precise P -> P * Q |-- P * R -> Q |-- R;
+  derives_precise: forall P Q, (P |-- Q) -> precise Q -> precise P;
+  precise_emp: precise emp;
+  precise_sepcon: forall P Q, precise Q -> precise P -> precise (P * Q)
+}.
+
+Class MapstoSepLog (Adr Val A: Type) {ND: NatDed A} {SL: SepLog A} {PSL: PreciseSepLog A} := mkMapstoSepLog {
+  mapsto: Adr -> Val -> A;
+  mapsto_conflict: forall a b b', mapsto a b * mapsto a b' |-- FF;
+  mapsto_precise: forall a b, precise (mapsto a b);
+  mapsto__precise: forall a, precise (EX b: Val, mapsto a b)
+}.
+
+Definition mapsto_ {Adr Val A: Type} {ND: NatDed A} {SL: SepLog A} {PSL: PreciseSepLog A} {MSL: MapstoSepLog Adr Val A} (a: Adr): A := EX b: Val, mapsto a b.
+
 Class OverlapSL (A: Type) {ND: NatDed A} {SL: SepLog A} := mkOverlapSL {
   ocon: A -> A -> A;
   ocon_emp: forall P, ocon P emp = P;
@@ -35,28 +68,3 @@ Module OconNotation.
 Notation "P ⊗ Q" := (ocon P Q) (at level 40, left associativity) : logic.
 End OconNotation.
 
-Class HONatDed (A: Type) {ND: NatDed A} := mkHONatDed {
-  allp_uncurry: forall (S T: Type) (P: S -> T -> A),
-    allp (fun s => allp (P s)) = allp (fun st => P (fst st) (snd st));
-  allp_curry: forall (S T: Type) (P: S * T -> A),
-    allp P = allp (fun s => allp (fun t => P (s, t)));
-  exp_uncurry: forall (S T: Type) (P: S -> T -> A),
-    exp (fun s => exp (P s)) = exp (fun st => P (fst st) (snd st));
-  exp_curry: forall (S T: Type) (P: S * T -> A),
-    exp P = exp (fun s => exp (fun t => P (s, t)));
-  allp_exp: forall (S T: Type) (P: S -> T -> A),
-    allp (fun s => exp (P s)) = exp (fun t: S -> T => allp (fun s => P s (t s)));
-  exp_allp: forall (S T: Type) (P: S -> T -> A),
-    exp (fun s => allp (P s)) |-- allp (fun t => exp (fun s => P s t))
-}.
-
-Class PreciseSepLog (A: Type) {ND: NatDed A} {SL: SepLog A} := mkPreciseSepLog {
-  precise: A -> Prop;
-  precise_spec: forall P Q R, precise P -> (P * Q) && (P * R) |-- P * (Q && R);
-  derives_precise: forall P Q, (P |-- Q) -> precise Q -> precise P
-}.
-
-Class MapstoSepLog (Adr Val A: Type) {ND: NatDed A} {SL: SepLog A} := mkMapstoSepLog {
-  mapsto: Adr -> Val -> A;
-  mapsto_conflict: forall a b b', mapsto a b * mapsto a b' |-- FF
-}.
