msl_ext/log_normalize.v
@@ -23,3 +23,45 @@ Proof.
   eapply allp_left.
   apply derives_refl.
 Qed.
+
+Lemma precise_wand_sepcon: forall {A: Type} {ND: NatDed A} {SL: SepLog A} {PSL: PreciseSepLog A} P Q, precise P -> P -* (P * Q) = Q.
+Proof.
+  intros.
+  apply pred_ext.
+  + apply precise_sepcon_cancel with P; auto.
+    apply modus_ponens_wand.
+  + apply wand_sepcon_adjoint.
+    rewrite sepcon_comm.
+    apply derives_refl.
+Qed.
+
+Lemma precise_andp_left: forall {A: Type} {ND: NatDed A} {SL: SepLog A} {PSL: PreciseSepLog A} P Q, precise P -> precise (P && Q).
+Proof.
+  intros.
+  apply derives_precise with P; auto.
+  apply andp_left1; auto.
+Qed.
+  
+Lemma precise_andp_right: forall {A: Type} {ND: NatDed A} {SL: SepLog A} {PSL: PreciseSepLog A} P Q, precise Q -> precise (P && Q).
+Proof.
+  intros.
+  apply derives_precise with Q; auto.
+  apply andp_left2; auto.
+Qed.
+
+Lemma exp_sepcon: forall {A: Type} {ND: NatDed A} {SL: SepLog A} {B} (P Q: B -> A), exp (P * Q) |-- exp P * exp Q.
+Proof.
+  intros.
+  apply exp_left; intro.
+  simpl.
+  apply sepcon_derives; apply (exp_right x); apply derives_refl.
+Qed.
+
+Lemma precise_exp_sepcon: forall {A: Type} {ND: NatDed A} {SL: SepLog A} {PSL: PreciseSepLog A} {B} (P Q: B -> A), precise (exp P) -> precise (exp Q) -> precise (exp (P * Q)).
+Proof.
+  intros.
+  eapply derives_precise.
+  + apply exp_sepcon.
+  + apply precise_sepcon; auto.
+Qed.
+
