msl_ext/msl_ext.v
@@ -49,16 +49,6 @@ Lemma precise_andp_right {A} {JA : Join A} {PA : Perm_alg A} {SA: Sep_alg A} {AG
   forall P Q, precise Q -> precise (P && Q).
 Proof. intros; intro; intros; destruct H0; destruct H1; generalize (H w w1 w2 H4 H5 H2 H3); tauto. Qed.
 
-Lemma precise_orp {A} {JA : Join A} {PA : Perm_alg A} {SA: Sep_alg A} {AG : ageable A} {AA: Age_alg A} :
-  forall (P Q: pred A), (forall w1 w2: A, ~ (P w1 /\ Q w2)) -> (precise P) -> precise Q -> precise (P || Q).
-Proof.
-  intros P Q Hfalse H H0; intro; intros.
-  destruct H1; destruct H2. generalize (H w w1 w2 H1 H2 H3 H4); tauto.
-  specialize (Hfalse w1 w2); destruct Hfalse; intuition.
-  specialize (Hfalse w2 w1); destruct Hfalse; intuition.
-  generalize (H0 w w1 w2 H1 H2 H3 H4); tauto.
-Qed.
-
 Lemma precise_sepcon {A} {JA : Join A} {PA : Perm_alg A} {SA: Sep_alg A} {AG : ageable A} {AA: Age_alg A} :
   forall P Q, precise Q -> precise P -> precise (P * Q).
 Proof.
